\newcommand{\A}[0]{\texttt{A}}
\newcommand{\C}[0]{\texttt{C}}
\newcommand{\G}[0]{\texttt{G}}
\newcommand{\U}[0]{\texttt{U}}

\documentclass{article}
\usepackage{enumitem}
\usepackage{amsmath}
\usepackage{amsfonts}
\title{Homework 1}
\author{Nathaniel Thomas \\ A17069898}
\begin{document}

\maketitle

\begin{enumerate}
	\item
	      \begin{enumerate}
		      \item $\{ \A\A, \A\A\A, \A\C\A, \C\A\A, \C\A, \C\C\A \}$
		      \item $\{ (\A, \A\A), (\C, \A\A), (\A, \A), (\C, \A), (\A, \C\A), (\C, \C\A)\}$
		      \item $\{ ((\A, \A), \C), ((\C, \C), \C), ((\A, \A), \A), ((\C, \C), \A) \}$
		      \item $\{ (-1, \A\A), (0, \A\A), (1, \A\A) \}$
		      \item $\{9, 10, 11, 12, 13, 14, 15\}$
		      \item $ \{ \A\U, \A\G, \C\U, \C\G, \U\U, \U\G, \G\U, \G\G \} $
	      \end{enumerate}
	\item
	      Basis Step:
	      \begin{align*}
		      \text{rnafunc} & :  S \to \mathbb{Z}^+                           \\
		      \text{If }     & b \in \{\A, \C\}      & \text{rnafunc}(b) & = 1 \\
		      \text{If }     & b \in \{\U, \G\}      & \text{rnafunc}(b) & = 0 \\
		      % \text{rnafunc}(\C) =  \text{rnafunc}(\G)                          & = 1 \\
		      % \text{rnafunc}(\lambda) = \text{rnafunc}(\A) = \text{rnafunc}(\U) & = 0 \\
	      \end{align*}
	      Recursive Step:
	      \begin{align*}
		       & \text{If } s \in S \text{ and } b \in \{\A, \C, \U, \G\} & \text{rnafunc}(sb) = \text{rnafunc}(s) + \text{rnafunc}(b)
		      % \text{rnafunc}(s) & =                                                                       \\
		      % V                 & = \{ \text{rnafunc}(a) + \text{rnafunc}(b) \mid ab = s \land |a| = 1 \} \\
		      %                   & \text{return } \sum_{x \in V} x                                         \\
	      \end{align*}
	\item
	      \begin{enumerate}
		      \item
		            \begin{align*}
			            dist(A, B) & = 3.4641016151377544 \\
			            dist(A, C) & = 2.6457513110645907 \\
			            dist(A, D) & = 4.0                \\
			            dist(B, C) & = 1.7320508075688772 \\
			            dist(B, D) & = 2.0                \\
			            dist(C, D) & = 3.3166247903554    \\
		            \end{align*}

		            The closest are Users B and C, and the farthest are users A and D.

		      \item
		            \begin{align*}
			            dot(A, A) & = (-1)^2 + 1^2 + (-1)^2 + 0^2 + 1^2 + 0^2 & = 4 \\
			            dot(B, B) & = 1^2 + 0^2 + 0^2 + 1^2 + (-1)^2 + 1^2    & = 4 \\
			            dot(C, C) & = 0^2 + 1^2 + (-1)^2 + 1^2 + (-1)^2 + 1^2 & = 5 \\
			            dot(D, D) & = 1^2 + (-1)^2 + 1^2 + 0^2 + (-1)^2 + 0^2 & = 4 \\
		            \end{align*}

		      \item
		            $$
			            \frac{dot((-1,1,-1,0,1,0), (1,-1,1,0,-1,0))}{
				            \sqrt{dot((-1,1,-1,0,1,0), (-1,1,-1,0,1,0))}
				            \sqrt{dot((1,-1,1,0,-1,0), (1,-1,1,0,-1,0))}
			            }
		            $$
		            $$
			            = \frac{-4}{\sqrt{4}\sqrt{4}} = -1
		            $$

		            The rating of User A for every movie is -1 times that for User D.

		      \item
		            The distance between two users tells us how large the cumulative difference
		            is for each movie. The cosine similarity tells us how much each user
		            has in common. I like the cosine similarity metric better because I think
		            it would be more useful for generating recommendations.

	      \end{enumerate}

	\item
	      \begin{enumerate}
		      \item dist(A, B) = 149.28496240412161
		      \item Colors E and F have dist(E, F) = 47.7283982551269
		      \item The distance formula is unreliable because the human eye does not
		            percieve changes in the R, G, and B components uniformly, but the distance
		            formula gives them equal weightings. A better way would be to scale the
		            squared difference between each entry by a constant that can be found to be
		            representative of human perception. \\

		            $$
			            betterdist((r_1, g_1, b_1), (r_2, g_2, b_2)) =
		            $$
		            $$
			            \sqrt{c_1(r_1 - r_2)^2 + c_2(g_1 - g_2)^2 + (b_1 - b_2)^2}
		            $$
	      \end{enumerate}

\end{enumerate}

\end{document}
